library/init/coe.lean
@@ -42,7 +42,7 @@ class HasCoeT (a : Sort u) (b : Sort v) :=
 (coe : a → b)
 
 class HasCoeToFun (a : Sort u) : Sort (max u (v+1)) :=
-(F : a → Sort v) (coe : Π x, F x)
+(F : a → Sort v) (coe : ∀ x, F x)
 
 class HasCoeToSort (a : Sort u) : Type (max u (v+1)) :=
 (S : Sort v) (coe : a → S)
@@ -59,7 +59,7 @@ class HasCoeToSort (a : Sort u) : Type (max u (v+1)) :=
 @[inline] def coeT {a : Sort u} {b : Sort v} [HasCoeT a b] : a → b :=
 @HasCoeT.coe a b _
 
-@[inline] def coeFnB {a : Sort u} [HasCoeToFun.{u, v} a] : Π x : a, HasCoeToFun.F.{u, v} x :=
+@[inline] def coeFnB {a : Sort u} [HasCoeToFun.{u, v} a] : ∀ x : a, HasCoeToFun.F.{u, v} x :=
 HasCoeToFun.coe
 
 /- User Level coercion operators -/
@@ -67,7 +67,7 @@ HasCoeToFun.coe
 @[reducible, inline] def coe {a : Sort u} {b : Sort v} [HasLiftT a b] : a → b :=
 liftT
 
-@[reducible, inline] def coeFn {a : Sort u} [HasCoeToFun.{u, v} a] : Π x : a, HasCoeToFun.F.{u, v} x :=
+@[reducible, inline] def coeFn {a : Sort u} [HasCoeToFun.{u, v} a] : ∀ x : a, HasCoeToFun.F.{u, v} x :=
 HasCoeToFun.coe
 
 @[reducible, inline] def coeSort {a : Sort u} [HasCoeToSort.{u, v} a] : a → HasCoeToSort.S.{u, v} a :=
