library/init/control/functor.lean
@@ -9,8 +9,8 @@ open Function
 universes u v
 
 class Functor (f : Type u → Type v) : Type (max (u+1) v) :=
-(map : Π {α β : Type u}, (α → β) → f α → f β)
-(mapConst : Π {α β : Type u}, α → f β → f α := fun α β => map ∘ const β)
+(map : ∀ {α β : Type u}, (α → β) → f α → f β)
+(mapConst : ∀ {α β : Type u}, α → f β → f α := fun α β => map ∘ const β)
 
 infixr <$> := Functor.map
 infixr <$  := Functor.mapConst
