library/init/data/option/instances.lean
@@ -8,11 +8,11 @@ import init.data.option.basic
 
 universes u v
 
-theorem Option.eqOfEqSome {α : Type u} : Π {x y : Option α}, (∀z, x = some z ↔ y = some z) → x = y
+theorem Option.eqOfEqSome {α : Type u} : ∀ {x y : Option α}, (∀z, x = some z ↔ y = some z) → x = y
 | none     none     h := rfl
 | none     (some z) h := Option.noConfusion ((h z).2 rfl)
 | (some z) none     h := Option.noConfusion ((h z).1 rfl)
 | (some z) (some w) h := Option.noConfusion ((h w).2 rfl) (congrArg some)
 
-theorem Option.eqNoneOfIsNone {α : Type u} : Π {o : Option α}, o.isNone → o = none
+theorem Option.eqNoneOfIsNone {α : Type u} : ∀ {o : Option α}, o.isNone → o = none
 | none h := rfl
